MIRification continued.

Exp.thy
@@ -6,82 +6,111 @@ section \<open>Semantics of Expressions\<close>
 
 text \<open>This section presents the big-step semantics of expressions.\<close>
 
-inductive place_sem ::
-  "gamma \<Rightarrow> heap \<Rightarrow> place \<Rightarrow> (address * tag) list * val \<Rightarrow> bool"
-  ("(_; _ \<turnstile> _ \<Down>\<^sub>p _)")
-where
-  Var: "\<Gamma> x = (a, t) \<Longrightarrow> \<Gamma>; H \<turnstile> Var x \<Down>\<^sub>p ([], Reference a t)" |
-  Deref: "\<lbrakk>\<Gamma>; H \<turnstile> p \<Down>\<^sub>p (refs, Reference a t); allocated H a\<rbrakk> \<Longrightarrow>
-          \<Gamma>; H \<turnstile> Deref p \<Down>\<^sub>p ((a, t) # refs, fst (H ! a))"
+text \<open>Introducing a locale here looks a good idea as it helps us formulate
+axioms among the heap access modifier. Expected axioms:
+\<^item> Modifier must be idempotent: \<^term>\<open>m p (m p H) = m p H\<close>.
+\<^item> Modifier must not allocate/deallocate a memory cell: \<^term>\<open>length (m p H) = length H\<close>.
+\<^item> The content is left intact: \<^term>\<open>fst ((m p H) ! a) = fst (H ! a)\<close>
+\<close>
 
-text \<open>The relation @{const place_sem} describes the semantics of places.
-\<^term>\<open>\<Gamma>; H \<turnstile> p \<Down>\<^sub>p (refs, v)\<close> means that a place expression \<^term>\<open>p\<close> evaluates to
-a value \<^term>\<open>v\<close> under the environment \<^term>\<open>\<Gamma>\<close> and \<^term>\<open>H\<close>, where \<^term>\<open>refs\<close> are
-the references used to retrieve the value (thus they need to be validated).\<close>
+type_synonym modifier = "(address * tag) \<Rightarrow> heap \<Rightarrow> heap option"
+fun write_access :: modifier where
+  "write_access (a, t) H =
+    (if writable H (a, t) then
+      let (v, ts) = H ! a in
+      Some (H[a := (v, kill t ts)])
+     else None)"
+fun read_access :: modifier where
+  "read_access (a, t) H =
+    (if readable H (a, t) then
+      let (v, ts) = H ! a in
+      Some (H[a := (v, kill t ts)])
+     else None)"
+
+inductive place_sem ::
+  "gamma \<Rightarrow> modifier \<Rightarrow> heap * place \<Rightarrow> heap * val \<Rightarrow> bool"
+  ("(_; _ \<turnstile> _ \<Down>\<^sub>p _)") for \<Gamma> m
+where
+  Var: "\<Gamma> x = (a, t) \<Longrightarrow> \<Gamma>; m \<turnstile> (H, Var x) \<Down>\<^sub>p (H, Reference a t)" |
+  Deref: "\<lbrakk>\<Gamma>; m \<turnstile> (H, p) \<Down>\<^sub>p (H', Reference a t); m (a, t) H' = Some H''\<rbrakk> \<Longrightarrow>
+          \<Gamma>; m \<turnstile> (H, Deref p) \<Down>\<^sub>p (H'', fst (H'' ! a))"
+
+text \<open>The relation @{const place_sem} describes the semantics of places
+with respect to a heap access modifier \<^term>\<open>m\<close>.
+\<^term>\<open>\<Gamma>; m \<turnstile> (H, p) \<Down>\<^sub>p (H', v)\<close> means that a place expression \<^term>\<open>p\<close> evaluates to
+a value \<^term>\<open>v\<close> under the environment \<^term>\<open>\<Gamma>\<close> and \<^term>\<open>H\<close>, while the access
+has changed the state of the heap to \<^term>\<open>H'\<close>.\<close>
+
+text \<open>We give a shorthand for read and write access to the place.\<close>
+
+abbreviation read_place_sem :: "gamma \<Rightarrow> heap * place \<Rightarrow> heap * val \<Rightarrow> bool"
+  ("(_ \<turnstile>\<^sub>r _ \<Down>\<^sub>p _)")
+  where
+  "\<Gamma> \<turnstile>\<^sub>r p \<Down>\<^sub>p v == \<Gamma>; read_access \<turnstile> p \<Down>\<^sub>p v"
+abbreviation write_place_sem :: "gamma \<Rightarrow> heap * place \<Rightarrow> heap * val \<Rightarrow> bool"
+  ("(_ \<turnstile>\<^sub>w _ \<Down>\<^sub>p _)")
+  where
+  "\<Gamma> \<turnstile>\<^sub>w p \<Down>\<^sub>p v == \<Gamma>; write_access \<turnstile> p \<Down>\<^sub>p v"
 
 (*<*)
 lemmas place_sem_cases = place_sem.cases[split_format(complete)]
 lemmas place_sem_induct = place_sem.induct[split_format(complete)]
 declare place_sem.intros[simp, intro]
 inductive_cases place_sem_inv[elim!]:
-  "\<Gamma>; H \<turnstile> Var x \<Down>\<^sub>p (refs, v)"
-  "\<Gamma>; H \<turnstile> Deref p \<Down>\<^sub>p (refs, v)"
+  "\<Gamma>; m \<turnstile> (H, Var x) \<Down>\<^sub>p (H', v)"
+  "\<Gamma>; m \<turnstile> (H, Deref p) \<Down>\<^sub>p (H', v)"
 (*>*)
 
+text \<open>Note that every operand is considered as a read access to the place.\<close>
+
 inductive operand_sem ::
-  "gamma \<Rightarrow> heap \<Rightarrow> operand \<Rightarrow> (address * tag) list * val \<Rightarrow> bool"
-  ("(_; _ \<turnstile> _ \<Down>\<^sub>o\<^sub>p _)")
+  "gamma \<Rightarrow> heap * operand \<Rightarrow> heap * val \<Rightarrow> bool"
+  ("(_ \<turnstile> _ \<Down>\<^sub>o\<^sub>p _)") for \<Gamma>
 where
-  Place: "\<Gamma>; H \<turnstile> p \<Down>\<^sub>p v \<Longrightarrow> \<Gamma>; H \<turnstile> Place p \<Down>\<^sub>o\<^sub>p v" |
-  Constant: "\<Gamma>; H \<turnstile> Constant v \<Down>\<^sub>o\<^sub>p ([], v)"
+  Place: "\<Gamma> \<turnstile>\<^sub>r (H, p) \<Down>\<^sub>p v \<Longrightarrow> \<Gamma> \<turnstile> (H, Place p) \<Down>\<^sub>o\<^sub>p v" |
+  Constant: "\<Gamma> \<turnstile> (H, Constant v) \<Down>\<^sub>o\<^sub>p (H, v)"
 
 (*<*)
 lemmas operand_sem_cases = operand_sem.cases[split_format(complete)]
 lemmas operand_sem_induct = operand_sem.induct[split_format(complete)]
 declare operand_sem.simps[simp, intro]
 inductive_cases operand_sem_inv[elim!]:
-  "\<Gamma>; H \<turnstile> Place p \<Down>\<^sub>o\<^sub>p v"
-  "\<Gamma>; H \<turnstile> Constant v \<Down>\<^sub>o\<^sub>p v'"
+  "\<Gamma> \<turnstile> (H, Place p) \<Down>\<^sub>o\<^sub>p v"
+  "\<Gamma> \<turnstile> (H, Constant v) \<Down>\<^sub>o\<^sub>p v'"
 (*>*)
 
 inductive rvalue_sem ::
-  "gamma * tags * heap * rvalue \<Rightarrow> tags * heap * val \<Rightarrow> bool" (infix "\<Down>" 65)
+  "gamma \<Rightarrow> tags * heap * rvalue \<Rightarrow> tags * heap * val \<Rightarrow> bool"
+  ("(_ \<turnstile> _ \<Down> _)") for \<Gamma>
 where
-  Use: "\<lbrakk>\<Gamma>; H \<turnstile> op \<Down>\<^sub>o\<^sub>p (refs, v); list_all (readable H) refs\<rbrakk>
-        \<Longrightarrow> (\<Gamma>, T, H, Use op) \<Down> (T, kill_all refs H, v)" |
-  Box: "\<lbrakk>\<Gamma>; H \<turnstile> op \<Down>\<^sub>o\<^sub>p (refs, v); p = length H; t = length T\<rbrakk>
-        \<Longrightarrow> (\<Gamma>, T, H, Box op) \<Down> (T @ [Unique], H @ [(v, [t])], Reference p t)" |
-  Ref: "\<lbrakk>\<Gamma>; H \<turnstile> p \<Down>\<^sub>p (refs, Reference a t); list_all (readable H) refs\<rbrakk>
-        \<Longrightarrow> (\<Gamma>, T, H, Ref p) \<Down> (T, kill_all refs H, Reference a t)" |
-  Reborrow: "\<lbrakk>\<Gamma>; H \<turnstile> p \<Down>\<^sub>p (refs, Reference a t); list_all (writable H) refs;
-              writable H (a, t); t' = length T;
-              H' = kill_all ((a, t) # refs) H; H' ! a = (v, ts)\<rbrakk>
-             \<Longrightarrow> (\<Gamma>, T, H, Reborrow p) \<Down> (T @ [Unique], H'[a := (v, ts @ [t'])] , Reference a t')" |
-  Plus: "\<lbrakk>\<Gamma>; H \<turnstile> lhs \<Down>\<^sub>o\<^sub>p (rl, VInt lhs'); \<Gamma>; H \<turnstile> rhs \<Down>\<^sub>o\<^sub>p (rr, VInt rhs');
-          list_all (readable H) rl; list_all (readable H) rr\<rbrakk>
-         \<Longrightarrow> (\<Gamma>, T, H, Plus lhs rhs) \<Down> (T, kill_all (rr @ rl) H, VInt (lhs' + rhs'))" |
-  Less: "\<lbrakk>\<Gamma>; H \<turnstile> lhs \<Down>\<^sub>o\<^sub>p (rl, VInt lhs'); \<Gamma>; H \<turnstile> rhs \<Down>\<^sub>o\<^sub>p (rr, VInt rhs');
-          list_all (readable H) rl; list_all (readable H) rr\<rbrakk>
-         \<Longrightarrow> (\<Gamma>, T, H, Less lhs rhs) \<Down> (T, kill_all (rr @ rl) H, VBool (lhs' < rhs'))" |
-  Not: "\<lbrakk>\<Gamma>; H \<turnstile> op \<Down>\<^sub>o\<^sub>p (refs, VBool v); list_all (readable H) refs\<rbrakk>
-         \<Longrightarrow> (\<Gamma>, T, H, Not op) \<Down> (T, kill_all refs H, VBool (\<not>v))" |
-  And: "\<lbrakk>\<Gamma>; H \<turnstile> lhs \<Down>\<^sub>o\<^sub>p (rl, VBool lhs'); \<Gamma>; H \<turnstile> rhs \<Down>\<^sub>o\<^sub>p (rr, VBool rhs');
-          list_all (readable H) rl; list_all (readable H) rr\<rbrakk>
-         \<Longrightarrow> (\<Gamma>, T, H, And lhs rhs) \<Down> (T, kill_all (rr @ rl) H, VBool (lhs' \<and> rhs'))"
+  Use: "\<Gamma> \<turnstile> (H, op) \<Down>\<^sub>o\<^sub>p (H', v) \<Longrightarrow> \<Gamma> \<turnstile> (T, H, Use op) \<Down> (T, H', v)" |
+  Box: "\<lbrakk>\<Gamma> \<turnstile> (H, op) \<Down>\<^sub>o\<^sub>p (H', v); p = length H'; t = length T\<rbrakk>
+        \<Longrightarrow> \<Gamma> \<turnstile> (T, H, Box op) \<Down> (T @ [Unique], H' @ [(v, [t])], Reference p t)" |
+  Ref: "\<Gamma> \<turnstile>\<^sub>w (H, p) \<Down>\<^sub>p (H', Reference a t) \<Longrightarrow> \<Gamma> \<turnstile> (T, H, Ref p) \<Down> (T, H', Reference a t)" |
+  Reborrow: "\<lbrakk>\<Gamma> \<turnstile>\<^sub>w (H, p) \<Down>\<^sub>p (H', Reference a t); writable H (a, t);
+              t' = length T; H' ! a = (v, ts)\<rbrakk>
+             \<Longrightarrow> \<Gamma> \<turnstile> (T, H, Reborrow p) \<Down> (T @ [Unique], H'[a := (v, ts @ [t'])], Reference a t')" |
+  Plus: "\<lbrakk>\<Gamma> \<turnstile> (H, lhs) \<Down>\<^sub>o\<^sub>p (H', VInt lhs'); \<Gamma> \<turnstile> (H', rhs) \<Down>\<^sub>o\<^sub>p (H'', VInt rhs')\<rbrakk>
+         \<Longrightarrow> \<Gamma> \<turnstile> (T, H, Plus lhs rhs) \<Down> (T, H'', VInt (lhs' + rhs'))" |
+  Less: "\<lbrakk>\<Gamma> \<turnstile> (H, lhs) \<Down>\<^sub>o\<^sub>p (H', VInt lhs'); \<Gamma> \<turnstile> (H', rhs) \<Down>\<^sub>o\<^sub>p (H'', VInt rhs')\<rbrakk>
+         \<Longrightarrow> \<Gamma> \<turnstile> (T, H, Less lhs rhs) \<Down> (T, H'', VBool (lhs' < rhs'))" |
+  Not: "\<Gamma> \<turnstile> (H, op) \<Down>\<^sub>o\<^sub>p (H', VBool v) \<Longrightarrow> \<Gamma> \<turnstile> (T, H, Not op) \<Down> (T, H', VBool (\<not>v))" |
+  And: "\<lbrakk>\<Gamma> \<turnstile> (H, lhs) \<Down>\<^sub>o\<^sub>p (H', VBool lhs'); \<Gamma> \<turnstile> (H', rhs) \<Down>\<^sub>o\<^sub>p (H'', VBool rhs')\<rbrakk>
+         \<Longrightarrow> \<Gamma> \<turnstile> (T, H, And lhs rhs) \<Down> (T, H'', VBool (lhs' \<and> rhs'))"
 
 (*<*)
 lemmas rvalue_sem_cases = rvalue_sem.cases[split_format(complete)]
 lemmas rvalue_sem_induct = rvalue_sem.induct[split_format(complete)]
 declare rvalue_sem.intros[simp, intro]
 inductive_cases rvalue_sem_inv[elim!]:
-  "(\<Gamma>, T, H, Use op) \<Down> (T', H', v)"
-  "(\<Gamma>, T, H, Box op) \<Down> (T', H', v)"
-  "(\<Gamma>, T, H, Ref p) \<Down> (T', H', v)"
-  "(\<Gamma>, T, H, Reborrow p) \<Down> (T', H', v)"
-  "(\<Gamma>, T, H, Plus lhs rhs) \<Down> (T', H', v)"
-  "(\<Gamma>, T, H, Less lhs rhs) \<Down> (T', H', v)"
-  "(\<Gamma>, T, H, Not op) \<Down> (T', H', v)"
-  "(\<Gamma>, T, H, And lhs rhs) \<Down> (T', H', v)"
+  "\<Gamma> \<turnstile> (T, H, Use op) \<Down> (T', H', v)"
+  "\<Gamma> \<turnstile> (T, H, Box op) \<Down> (T', H', v)"
+  "\<Gamma> \<turnstile> (T, H, Ref p) \<Down> (T', H', v)"
+  "\<Gamma> \<turnstile> (T, H, Reborrow p) \<Down> (T', H', v)"
+  "\<Gamma> \<turnstile> (T, H, Plus lhs rhs) \<Down> (T', H', v)"
+  "\<Gamma> \<turnstile> (T, H, Less lhs rhs) \<Down> (T', H', v)"
+  "\<Gamma> \<turnstile> (T, H, Not op) \<Down> (T', H', v)"
+  "\<Gamma> \<turnstile> (T, H, And lhs rhs) \<Down> (T', H', v)"
 (*>*)
 
 text \<open>
@@ -101,8 +130,6 @@ returning a reference pointing to the slot with a fresh tag.
 \end{framed}
 
 Next, {\sc{Use}} and {\sc{Ref}} rules allow us to read the content through a place (or give a constant).
-The validity of the access is checked by @{const_typ readable}.
-Moreover, they invalidate all descendant references to establish the uniqueness.
 
 \begin{framed}
 \centering
@@ -125,18 +152,22 @@ reference as the last two element.
 
 text \<open>We can prove that the semantics of expressions is deterministic.\<close>
 
-lemma place_sem_det: "\<Gamma>; H \<turnstile> p \<Down>\<^sub>p (refs, v) \<Longrightarrow> \<Gamma>; H \<turnstile> p \<Down>\<^sub>p (refs', v') \<Longrightarrow> (refs', v') = (refs, v)"
-proof (induction arbitrary: refs' v' rule: place_sem.induct)
-  case (Var \<Gamma> x a t H)
-  then show ?case by auto
+lemma place_sem_det: "\<Gamma>; m \<turnstile> p \<Down>\<^sub>p v \<Longrightarrow> \<Gamma>; m \<turnstile> p \<Down>\<^sub>p v' \<Longrightarrow> v' = v"
+proof (induction arbitrary: v' rule: place_sem.induct)
+  case (Var x a t H)
+  then show ?case
+    by (metis Pair_inject place_sem_inv(1) surj_pair)
 next
-  case (Deref \<Gamma> H p refs a t)
-  then show ?case by blast
+  case (Deref m H p H' a t H'')
+  then show ?case
+    by (smt Pair_inject option.inject place_sem_inv(2) surj_pair val.inject(3))
 qed
-lemmas place_sem_det' = place_sem_det[split_format(complete)]
+lemma place_sem_det': "\<Gamma>; m \<turnstile> (H, p) \<Down>\<^sub>p (H', v') \<Longrightarrow> \<Gamma>; m \<turnstile> (H, p) \<Down>\<^sub>p (H'', v'')
+  \<Longrightarrow> (H'', v'') = (H', v')"
+  using place_sem_det by auto
 
-lemma operand_sem_det: "\<Gamma>; H \<turnstile> op \<Down>\<^sub>o\<^sub>p (refs, v) \<Longrightarrow> \<Gamma>; H \<turnstile> op \<Down>\<^sub>o\<^sub>p (refs', v') \<Longrightarrow> (refs', v') = (refs, v)"
-proof (induction arbitrary: refs' v' rule: operand_sem.induct)
+lemma operand_sem_det: "\<Gamma> \<turnstile> op \<Down>\<^sub>o\<^sub>p v \<Longrightarrow> \<Gamma> \<turnstile> op \<Down>\<^sub>o\<^sub>p v' \<Longrightarrow> v' = v"
+proof (induction arbitrary: v' rule: operand_sem.induct)
   case (Place \<Gamma> H p v)
   then show ?case
     by (metis operand_sem_inv(1) place_sem_det' surj_pair)
@@ -144,151 +175,149 @@ next
   case (Constant \<Gamma> H v)
   then show ?case by blast
 qed
-lemmas operand_sem_det' = operand_sem_det[split_format(complete)]
+lemma operand_sem_det': "\<Gamma> \<turnstile> (H, op) \<Down>\<^sub>o\<^sub>p (H', v') \<Longrightarrow> \<Gamma> \<turnstile> (H, op) \<Down>\<^sub>o\<^sub>p (H'', v'')
+  \<Longrightarrow> (H'', v'') = (H', v')"
+  using operand_sem_det by blast
 
-lemma rvalue_sem_det: "(\<Gamma>, T, H, rv) \<Down> (T', H', v') \<Longrightarrow> (\<Gamma>, T, H, rv) \<Down> (T'', H'', v'')
+lemma rvalue_sem_det: "\<Gamma> \<turnstile> (T, H, rv) \<Down> (T', H', v') \<Longrightarrow> \<Gamma> \<turnstile> (T, H, rv) \<Down> (T'', H'', v'')
   \<Longrightarrow> (T'', H'', v'') = (T', H', v')"
-proof (induction rule: rvalue_sem_induct)
-  case (Use \<Gamma> H op refs v T)
-  show "(T'', H'', v'') = (T, kill_all refs H, v)"
-  proof (rule rvalue_sem_inv(1))
-    fix refs'
-    assume op: "(\<exists>p. op = Place p \<and> (\<Gamma>; H \<turnstile> p \<Down>\<^sub>p (refs', v''))) \<or> op = Constant v'' \<and> refs' = []"
-    then have "\<Gamma>; H \<turnstile> op \<Down>\<^sub>o\<^sub>p (refs', v'')" by simp
-    then have "refs' = refs" and "v'' = v" using Use.hyps(1) operand_sem_det' by auto
-    then show "(T'', H'', v'') = (T, kill_all refs H, v)"
-      using Use.prems op place_sem_det' by blast
-  next
-    show "(\<Gamma>, T, H, Use op) \<Down> (T'', H'', v'')" using Use.prems by auto
-  qed
+proof (induction arbitrary: T'' H'' v'' rule: rvalue_sem_induct)
+  case (Use H op H' v T)
+  then show ?case using operand_sem_det' by fastforce
 next
-  case (Box \<Gamma> H op refs v p t T)
-  then show ?case using place_sem_det' by auto
+  case (Box H op H' v p t T)
+  then show ?case using place_sem_det' by blast
 next
-  case (Ref \<Gamma> H p refs a t T)
-  then show ?case using place_sem_det' by fastforce
+  case (Ref H p H' a t T)
+  then show ?case using place_sem_det' by blast
 next
-  case (Reborrow \<Gamma> H p refs a t t' T H' v ts)
-  show "(T'', H'', v'') = (T @ [Unique], H'[a := (v, ts @ [t'])], Reference a t')"
+  case (Reborrow H p H' a t t' T v ts)
+  show ?case
   proof (rule rvalue_sem_inv(4))
-    show "(\<Gamma>, T, H, Reborrow p) \<Down> (T'', H'', v'')" using Reborrow.prems by simp
+    show "\<Gamma> \<turnstile> (T, H, Reborrow p) \<Down> (T'', H'', v'')" using Reborrow.prems by simp
   next
-    fix refsa aa ta va tsa
-    let ?kill = "(case kill_all refsa H ! aa of (va, tsa) \<Rightarrow> (kill_all refsa H)[aa := (va, kill ta tsa)])"
-    assume "\<Gamma>; H \<turnstile> p \<Down>\<^sub>p (refsa, Reference aa ta)"
-    then have "refsa = refs \<and> aa = a \<and> ta = t" using Reborrow.hyps place_sem_det' by blast
-    then have "refsa = refs" and "aa = a" and "ta = t" by auto
-    moreover assume "?kill ! aa = (va, tsa)"
-    then have "va = v" and "tsa = ts" using Reborrow.hyps calculation by auto
-    moreover assume "H'' = ?kill[aa := (va, tsa @ [length T])]"
-    then have "H'' = H'[a := (v, ts @ [t'])]" by (simp add: Reborrow.hyps calculation)
+    fix H'a aa ta va tsa
+    assume "\<Gamma> \<turnstile>\<^sub>w (H, p) \<Down>\<^sub>p (H'a, Reference aa ta)"
+    then have "H'a = H' \<and> aa = a \<and> ta = t" using Reborrow.hyps place_sem_det by fastforce
+    moreover assume "H'a ! aa = (va, tsa)"
+    then have "va = v \<and> tsa = ts" using Reborrow.hyps calculation by auto
+    moreover assume "H'' = H'a[aa := (va, tsa @ [length T])]"
+    then have "H'' = H'a[a := (v, ts @ [t'])]" using Reborrow.hyps calculation by simp
     moreover assume "v'' = Reference aa (length T)"
     then have "v'' = Reference a t'" using Reborrow.hyps calculation by simp
-    ultimately show ?thesis using Reborrow.prems by auto
+    moreover assume "T'' = T @ [Unique]"
+    thus ?thesis using calculation by simp
   qed
 next
-  case (Plus \<Gamma> H lhs rl lhs' rhs rr rhs' T)
-  show "(T'', H'', v'') = (T, kill_all (rr @ rl) H, VInt (lhs' + rhs'))"
+  case (Plus H lhs H' lhs' rhs He rhs' T)
+  show ?case
   proof (rule rvalue_sem_inv(5))
-    show "(\<Gamma>, T, H, Plus lhs rhs) \<Down> (T'', H'', v'')" using Plus.prems by simp
+    show "\<Gamma> \<turnstile> (T, H, Plus lhs rhs) \<Down> (T'', H'', v'')" using Plus.prems by simp
   next
-    fix rla lhs'a rra rhs'a
-    assume opl: "(\<exists>p. lhs = Place p \<and> (\<Gamma>; H \<turnstile> p \<Down>\<^sub>p (rla, VInt lhs'a))) \<or>
-            lhs = Constant (VInt lhs'a) \<and> rla = []" and
-           opr: "(\<exists>p. rhs = Place p \<and> (\<Gamma>; H \<turnstile> p \<Down>\<^sub>p (rra, VInt rhs'a))) \<or>
-            rhs = Constant (VInt rhs'a) \<and> rra = []"
-    then have "\<Gamma>; H \<turnstile> lhs \<Down>\<^sub>o\<^sub>p (rla, VInt lhs'a)" and "\<Gamma>; H \<turnstile> rhs \<Down>\<^sub>o\<^sub>p (rra, VInt rhs'a)" by auto
-    then have "rla = rl \<and> lhs'a = lhs' \<and> rra = rr \<and> rhs'a = rhs'"
-      using Plus.hyps operand_sem_det' by blast
-    then have "rla = rl" and "lhs'a = lhs'" and "rra = rr" and "rhs'a = rhs'" by auto
-    moreover assume "H'' = kill_all rra (kill_all rla H)" and "v'' = VInt (lhs'a + rhs'a)"
-    then have "H'' = kill_all (rr @ rl) H" and "v'' = VInt (lhs' + rhs')"
-      using calculation foldr_append by auto
-    ultimately show ?thesis using Plus.prems by auto
+    fix H'a lhs'a rhs'a
+    assume "(\<exists>p. lhs = Place p \<and> (\<Gamma> \<turnstile>\<^sub>r (H, p) \<Down>\<^sub>p (H'a, VInt lhs'a)))
+            \<or> lhs = Constant (VInt lhs'a) \<and> H'a = H"
+    then have "lhs'a = lhs' \<and> H'a = H'" using Plus.hyps operand_sem_det' by fastforce
+    moreover
+    assume "(\<exists>p. rhs = Place p \<and> (\<Gamma> \<turnstile>\<^sub>r (H'a, p) \<Down>\<^sub>p (H'', VInt rhs'a)))
+            \<or> rhs = Constant (VInt rhs'a) \<and> H'' = H'a"
+    then have "rhs'a = rhs' \<and> He = H''"
+      using Plus.hyps calculation operand_sem_det' by fastforce
+    moreover assume "v'' = VInt (lhs'a + rhs'a)"
+    thus ?thesis using calculation Plus.prems by auto
   qed
 next
-  case (Less \<Gamma> H lhs rl lhs' rhs rr rhs' T)
-  show "(T'', H'', v'') = (T, kill_all (rr @ rl) H, VBool (lhs' < rhs'))"
+  case (Less H lhs H' lhs' rhs He rhs' T)
+  show ?case
   proof (rule rvalue_sem_inv(6))
-    show "(\<Gamma>, T, H, Less lhs rhs) \<Down> (T'', H'', v'')" using Less.prems by simp
+    show "\<Gamma> \<turnstile> (T, H, Less lhs rhs) \<Down> (T'', H'', v'')" using Less.prems by simp
   next
-    fix rla lhs'a rra rhs'a
-    assume opl: "(\<exists>p. lhs = Place p \<and> (\<Gamma>; H \<turnstile> p \<Down>\<^sub>p (rla, VInt lhs'a))) \<or>
-            lhs = Constant (VInt lhs'a) \<and> rla = []" and
-           opr: "(\<exists>p. rhs = Place p \<and> (\<Gamma>; H \<turnstile> p \<Down>\<^sub>p (rra, VInt rhs'a))) \<or>
-            rhs = Constant (VInt rhs'a) \<and> rra = []"
-    then have "\<Gamma>; H \<turnstile> lhs \<Down>\<^sub>o\<^sub>p (rla, VInt lhs'a)" and "\<Gamma>; H \<turnstile> rhs \<Down>\<^sub>o\<^sub>p (rra, VInt rhs'a)" by auto
-    then have "rla = rl \<and> lhs'a = lhs' \<and> rra = rr \<and> rhs'a = rhs'"
-      using Less.hyps operand_sem_det' by blast
-    then have "rla = rl" and "lhs'a = lhs'" and "rra = rr" and "rhs'a = rhs'" by auto
-    moreover assume "H'' = kill_all rra (kill_all rla H)" and "v'' = VBool (lhs'a < rhs'a)"
-    then have "H'' = kill_all (rr @ rl) H" and "v'' = VBool (lhs' < rhs')"
-      using calculation foldr_append by auto
-    ultimately show ?thesis using Less.prems by auto
+    fix H'a lhs'a rhs'a
+    assume "(\<exists>p. lhs = Place p \<and> (\<Gamma> \<turnstile>\<^sub>r (H, p) \<Down>\<^sub>p (H'a, VInt lhs'a)))
+            \<or> lhs = Constant (VInt lhs'a) \<and> H'a = H"
+    then have "lhs'a = lhs' \<and> H'a = H'" using Less.hyps operand_sem_det' by fastforce
+    moreover
+    assume "(\<exists>p. rhs = Place p \<and> (\<Gamma> \<turnstile>\<^sub>r (H'a, p) \<Down>\<^sub>p (H'', VInt rhs'a)))
+            \<or> rhs = Constant (VInt rhs'a) \<and> H'' = H'a"
+    then have "rhs'a = rhs' \<and> He = H''"
+      using Less.hyps calculation operand_sem_det' by fastforce
+    moreover assume "v'' = VBool (lhs'a < rhs'a)"
+    thus ?thesis using calculation Less.prems by auto
   qed
 next
-  case (Not \<Gamma> H op refs v T)
-  show "(T'', H'', v'') = (T, kill_all refs H, VBool (\<not>v))"
+  case (Not H op H' v T)
+  show ?case
   proof (rule rvalue_sem_inv(7))
-    fix refsa va
-    assume "(\<exists>p. op = Place p \<and> (\<Gamma>; H \<turnstile> p \<Down>\<^sub>p (refsa, VBool va))) \<or> op = Constant (VBool va) \<and> refsa = []"
-    then show "(T'', H'', v'') = (T, kill_all refs H, VBool (\<not>v))"
-      using Not.prems Not.hyps operand_sem_det' place_sem_det' by blast
+    show "\<Gamma> \<turnstile> (T, H, Not op) \<Down> (T'', H'', v'')" using Not.prems by simp
   next
-    show "(\<Gamma>, T, H, Not op) \<Down> (T'', H'', v'')" using Not.prems by simp
+    fix va
+    assume "(\<exists>p. op = Place p \<and> (\<Gamma> \<turnstile>\<^sub>r (H, p) \<Down>\<^sub>p (H'', VBool va)))
+            \<or> op = Constant (VBool va) \<and> H'' = H"
+    then have "H'' = H' \<and> va = v" using Not.hyps operand_sem_det' by fastforce
+    moreover assume "T'' = T" and "v'' = VBool (\<not>va)"
+    thus ?thesis by (simp add: calculation)
   qed
 next
-  case (And \<Gamma> H lhs rl lhs' rhs rr rhs' T)
-  show "(T'', H'', v'') = (T, kill_all (rr @ rl) H, VBool (lhs' \<and> rhs'))"
+  case (And H lhs H' lhs' rhs He rhs' T)
+  show ?case
   proof (rule rvalue_sem_inv(8))
-    show "(\<Gamma>, T, H, And lhs rhs) \<Down> (T'', H'', v'')" using And.prems by simp
+    show "\<Gamma> \<turnstile> (T, H, And lhs rhs) \<Down> (T'', H'', v'')" using And.prems by simp
   next
-    fix rla lhs'a rra rhs'a
-    assume opl: "(\<exists>p. lhs = Place p \<and> (\<Gamma>; H \<turnstile> p \<Down>\<^sub>p (rla, VBool lhs'a))) \<or>
-            lhs = Constant (VBool lhs'a) \<and> rla = []" and
-           opr: "(\<exists>p. rhs = Place p \<and> (\<Gamma>; H \<turnstile> p \<Down>\<^sub>p (rra, VBool rhs'a))) \<or>
-            rhs = Constant (VBool rhs'a) \<and> rra = []"
-    then have "\<Gamma>; H \<turnstile> lhs \<Down>\<^sub>o\<^sub>p (rla, VBool lhs'a)" and "\<Gamma>; H \<turnstile> rhs \<Down>\<^sub>o\<^sub>p (rra, VBool rhs'a)" by auto
-    then have "rla = rl \<and> lhs'a = lhs' \<and> rra = rr \<and> rhs'a = rhs'"
-      using And.hyps operand_sem_det' by blast
-    then have "rla = rl" and "lhs'a = lhs'" and "rra = rr" and "rhs'a = rhs'" by auto
-    moreover assume "H'' = kill_all rra (kill_all rla H)" and "v'' = VBool (lhs'a \<and> rhs'a)"
-    then have "H'' = kill_all (rr @ rl) H" and "v'' = VBool (lhs' \<and> rhs')"
-      using calculation foldr_append by auto
-    ultimately show ?thesis using And.prems by auto
+    fix H'a lhs'a rhs'a
+    assume "(\<exists>p. lhs = Place p \<and> (\<Gamma> \<turnstile>\<^sub>r (H, p) \<Down>\<^sub>p (H'a, VBool lhs'a)))
+            \<or> lhs = Constant (VBool lhs'a) \<and> H'a = H"
+    then have "lhs'a = lhs' \<and> H'a = H'" using And.hyps operand_sem_det' by fastforce
+    moreover
+    assume "(\<exists>p. rhs = Place p \<and> (\<Gamma> \<turnstile>\<^sub>r (H'a, p) \<Down>\<^sub>p (H'', VBool rhs'a)))
+            \<or> rhs = Constant (VBool rhs'a) \<and> H'' = H'a"
+    then have "rhs'a = rhs' \<and> He = H''"
+      using And.hyps calculation operand_sem_det' by fastforce
+    moreover assume "v'' = VBool (lhs'a \<and> rhs'a)"
+    thus ?thesis using calculation And.prems by auto
   qed
 qed
 
 text \<open>The following lemmas are sanity checks of the semantics.
-We must be able to write through the references retrieved by {\sc{Box}} and {\sc{Reborrow}}\<close>
+We must be able to write through the references retrieved by {\sc{Box}} and {\sc{Reborrow}} rules.\<close>
 
-lemma box__writable: "(\<Gamma>, T, H, Box e) \<Down> (T', H', Reference a t) \<Longrightarrow> writable H' (a, t)"
+lemma box_writable: "\<Gamma> \<turnstile> (T, H, Box e) \<Down> (T', H', Reference a t) \<Longrightarrow> writable H' (a, t)"
   by auto
 
-lemma reborrow__writable: "(\<Gamma>, T, H, Reborrow p) \<Down> (T', H', Reference a t) \<Longrightarrow> writable H' (a, t)"
-proof (rule rvalue_sem_inv(4))
-  assume "(\<Gamma>, T, H, Reborrow p) \<Down> (T', H', Reference a t)"
-  then show "(\<Gamma>, T, H, Reborrow p) \<Down> (T', H', Reference a t)" by auto
+lemma wa_preserve_length: "write_access at H = Some H' \<Longrightarrow> length H' = length H"
+  by (smt kill_heap.simps kill_preserve_length option.distinct(1)
+          option.sel prod.case_eq_if write_access.elims)
+
+lemma write_preserve_length: "\<Gamma> \<turnstile>\<^sub>w p \<Down>\<^sub>p v \<Longrightarrow> length (fst p) = length (fst v)"
+proof (induction rule: place_sem.induct)
+  case (Var x a t H)
+  then show ?case by simp
 next
-  fix refsa aa ta va tsa
-  let ?kill = "(case kill_all refsa H ! aa of (va, tsa) \<Rightarrow> (kill_all refsa H)[aa := (va, kill ta tsa)])"
-  assume "H' = ?kill[aa := (va, tsa @ [length T])]"
-    and "aa < length H"
-    and "?kill ! aa = (va, tsa)"
-  then have "H' ! aa = (va, tsa @ [length T])"
-    by (metis (no_types, lifting) kill_all_preserve_length length_list_update
-      nth_list_update_eq prod.case_eq_if)
-  moreover assume "Reference a t = Reference aa (length T)"
-  then have "aa = a" and "t = length T" by auto
-  ultimately have alen: "a < length H" and elem: "H' ! a = (va, tsa @ [t])"
-    using \<open>aa < length H\<close> by auto
+  case (Deref H p H' a t H'')
+  assume "write_access (a, t) H' = Some H''"
+  then have "length H'' = length H'" using wa_preserve_length by blast
+  moreover
+  assume "length (fst (H, p)) = length (fst (H', Reference a t))"
+  then have "length H = length H'" by simp
+  ultimately have "length H'' = length H" by simp
+  thus ?case by simp
+qed
 
-  assume "H' = ?kill[aa := (va, tsa @ [length T])]"
-  then have alen': "a < length H'"
-    using alen kill_all_preserve_length kill_preserve_length by force
+lemma reborrow_writable: "\<Gamma> \<turnstile> (T, H, Reborrow p) \<Down> (T', H', Reference a t) \<Longrightarrow> writable H' (a, t)"
+proof (rule rvalue_sem_inv(4))
+  assume "\<Gamma> \<turnstile> (T, H, Reborrow p) \<Down> (T', H', Reference a t)"
+  then show "\<Gamma> \<turnstile> (T, H, Reborrow p) \<Down> (T', H', Reference a t)" by auto
+next
+  fix H'a aa ta va tsa
+  assume "Reference a t = Reference aa (length T)"
+  then have "aa = a" and "length T = t" by auto
 
-  have "t \<in> set (snd (H' ! a))" by (simp add: elem)
-  with alen' show ?thesis by auto
+  assume "\<Gamma> \<turnstile>\<^sub>w (H, p) \<Down>\<^sub>p (H'a, Reference aa ta)"
+  then have "length H'a = length H" using write_preserve_length by auto
+  moreover assume "aa < length H" then have "aa < length H'a" using calculation by simp
+  moreover assume "H' = H'a[aa := (va, tsa @ [length T])]"
+  then have "H' ! a = (va, tsa @ [t])" and "length H' = length H'a"
+    using \<open>aa < length H\<close> \<open>aa = a\<close> \<open>length T = t\<close> calculation by auto
+  thus ?thesis using \<open>aa = a\<close> \<open>aa < length H'a\<close> by auto
 qed
 
 end
